Prove STLC w/ dependent substitution calculus wf

src/named/STLC.v
@@ -1,24 +1,18 @@
-
-Require Import mathcomp.ssreflect.all_ssreflect.
 Set Implicit Arguments.
-Unset Strict Implicit.
-Unset Printing Implicit Defensive.
 Set Bullet Behavior "Strict Subproofs".
 
-
-From Ltac2 Require Import Ltac2.
-Set Default Proof Mode "Classic".
+Require Import String List.
+Import ListNotations.
+Open Scope string.
+Open Scope list.
 From Utils Require Import Utils.
-From Named Require Import Exp.
-From Named Require ICore.
-From Named Require Import Subst Tactics Decidable.
-Import ICore.IndependentJudgment Exp.Notations ARule.Notations.
-Require Import String.
+From Named Require Import Core Elab Matches Subst.
+Import Core.Notations.
 
-Set Default Proof Mode "Ltac2".
+Require Coq.derive.Derive.
 
 Definition stlc :=
-  [::[:> "G" : #"env", "A" : #"ty" %"G", "B" : #"ty" %"G",
+  [[:> "G" : #"env", "A" : #"ty" %"G", "B" : #"ty" %"G",
       "e" : #"el" (#"ext" %"G" %"A") (#"ty_subst" #"wkn" %"B"),
       "G'" : #"env",
       "g" : #"sub" %"G'" %"G"
@@ -78,519 +72,254 @@ Definition stlc :=
 
 Import OptionMonad.
 
-Section InferSub.
 
-  Context (subst_lang_el_ty : ctx -> exp (*G*) -> exp (*e*) -> option exp).
-
-  
-  Fixpoint sub_decompose' g f : option exp :=
-    if f == g then do ret {{e #"id"}}
-    else match f with
-         | con "cmp" [:: h; f'] =>
-           do ret {{e #"cmp" {sub_decompose g f'} {h} }}
-         | _ => None
-         end.
-  
-  Fixpoint sub_decompose g f : option exp :=
-    match g with
-    | con "cmp" [:: h; g'] =>
-      do g'_minus_f <- sub_decompose g' f;
-      res <- sub_decompose h (g'_minus_f);
-           ret res
-    | _ => sub_decompose' g f
-    end.
-
-  Definition ty_decompose g A :=
-    if g == {{e #"id"}} then do ret A
-    else match A with
-         | con "ty_subst" [:: A; g'] =>
-           do g'_minus_g <- sub_decompose g g';
-           ret {{e #"ty_subst" {g'_minus_g} {A} }}
-         | _ => None
-         end.
-
-  Fixpoint cat_lang_sub_r c e G_l : option exp :=
-    match e with
-    | con "id" [::] => G_l
-    | con "cmp" [:: g; f] =>
-      let G_lf := cat_lang_sub_r c f G_l in
-      let G_lg := cat_lang_sub_r c g G_lf in
-      G_lg
-    | con "wkn" [::] =>
-      match G_l with
-      | con "ext" [:: _;G_r] => G_r
-      | _ => {{e #"ERR"}}
-      end
-    | con "snoc" [:: e; f] =>
-      let G' := cat_lang_sub_r c f G_l in
-      let Af := subst_lang_el_ty c G' e in
-      {{e #"ext" {G'} {ty_decompose f Af} }}
-    | var x =>
-      match named_list_lookup {{s #"ERR"}} c x with
-      | scon "sub" [:: G; _] => G
-      | _ => {{e #"ERR"}}
-      end
-    | _ => {{e #"ERR"}}
-    end.
-
-End InferSub.
-  
-Fixpoint subst_lang_el_ty c G e : exp :=
-  match e,G with
-  | var x,_ => 
-    match named_list_lookup {{s #"ERR not in c"}} c x with
-    | scon "el" [:: t; _] => t
-    | _ => {{e #"ERR sort from c not in subst lang"}}
-    end
-  | con "hd" [::], con "ext" [:: A; G'] =>
-    {{e #"ty_subst" #"wkn" %"A" }}
-  | con "el_subst" [:: e'; g], _ =>
-    let G' := cat_lang_sub_r subst_lang_el_ty c g G in
-    let A := subst_lang_el_ty c G' e' in
-    {{e #"ty_subst" {g} {A} }}
-  | con "lambda" [:: e'; A], _ =>
-    let Bwkn := subst_lang_el_ty c {{e #"ext" {G} {A} }} e' in
-    {{e #"->" {A} {ty_decompose {{e#"wkn"}} Bwkn} }}
-  | con "app" [:: e'; e], _ =>
-    match subst_lang_el_ty c G e with
-    | con "->" [:: B; _] => B
-    | _ => {{e #"ERR: bad app"}}
-    end
-  | _, _ => {{e #"ERR: not in subst lang" }}
-  end.
-
-
-Instance rec_stlc : LangRecognize stlc :=
-  {  le_sort_dec := generic_sort_dec_fuel 10 stlc;
-    decide_le_sort := @generic_decide_le_sort 10 stlc;
-    term_args_elab c s name t := 
-      match name, t, s with
-      | "app", scon "el" [:: T; G], [:: e'; e] =>
-        match subst_lang_el_ty c G e with
-        | con "->" [:: B; A] => [:: e'; e; B; A; G]
-        | _ => [:: e';e; {{e #"ERR: bad app elab"}}]
-        end          
-      | "lambda", scon "el" [:: T; G], [:: e; A] =>
-        let T' := term_par_step_n stlc T 100 in
-        match T' with
-        | con "->" [:: B; _] =>
-          [:: e; B; A; G]
-        | _ => [:: {{e #"ERR"}}]
-        end
-      | "->", scon "ty" [:: G], [:: t'; t] => [:: t'; t; G]
-      | "forget", scon "sub" [:: _; G],_ => [:: G]
-      | "id", scon "sub" [:: _; G],_ => [:: G]
-      | "cmp", scon "sub" [:: G3; G1], [:: g; f] =>
-        let G2 := cat_lang_sub_r subst_lang_el_ty c f G1 in
-        [:: g; f; G3; G2; G1]
-      | "ty_subst", scon "ty" [:: G], [:: A; g] =>
-        let G' := cat_lang_sub_r subst_lang_el_ty c g G in
-        [:: A; g; G'; G]
-      | "el_subst", scon "el" [:: _; G], [:: e; g] =>
-        let G' := cat_lang_sub_r subst_lang_el_ty c g G in
-        let A := subst_lang_el_ty c G' e in
-        [:: e; A; g; G'; G]
-      | "snoc", scon "sub" [:: con "ext" [:: A; G']; G], [:: e; g] =>
-        [:: e; g; A; G'; G]
-      | "wkn", scon "sub" [:: G; con "ext" [:: A; _]], [::] =>
-        [:: A; G]
-      | "hd", scon "el" [:: _; con "ext" [:: A; G]], [::] =>
-        [:: A; G]
-      | _,_,_ => s
-      end%string;
-    sort_args_elab c s _ := s
-  }.
-
-Ltac2 rec break_forall_goal ():=
-  first [ apply List.Forall_nil
-        | apply List.Forall_cons > [| break_forall_goal()]].
-
-  
-Lemma stlc_wf : wf_lang stlc.
+Derive stlc_elab
+       SuchThat (elab_lang stlc stlc_elab)
+       As stlc_wf.
 Proof.
-  apply (decide_wf_lang (fuel:=100)).
-  match! goal with
-    [|-dm_remaining_goals _ ?comp] =>
-    let e := Std.eval_vm None comp in
-    Message.print (Message.of_constr e)
-  end.
-  ().
-  break_forall_goal ().
-  constructor.
-  apply (@decide_wf_lang _ _ 100).
-  next_goal().
+  
+  setup_elab_lang_proof.
+
+  solve [ break_elab_rule ].
+  solve [ break_elab_rule ].
+  solve [ break_elab_rule ].
+  solve [ break_elab_rule ].
+  solve [ break_elab_rule ].
+  solve [ break_elab_rule ].
+  solve [ break_elab_rule ].
+  solve [ break_elab_rule ].
+  solve [ break_elab_rule ].
+  solve [ break_elab_rule ].
+  solve [ break_elab_rule ].
+  solve [ break_elab_rule ].
+  solve [ break_elab_rule ].
+  solve [ break_elab_rule ].
+  solve [ break_elab_rule ].
+  solve [ break_elab_rule ].
+  solve [ break_elab_rule ].
+  solve [ break_elab_rule ].
+  solve [ break_elab_rule ].
+  solve [ break_elab_rule ].
+  solve [ break_elab_rule ].
+  solve [ break_elab_rule ].
+  solve [ break_elab_rule ].
+  solve [ break_elab_rule ].
+  solve [ break_elab_rule ].
+  solve [ break_elab_rule ].
+  solve [ break_elab_rule ].
+  solve [ break_elab_rule ].
+  solve [ break_elab_rule ].
+  solve [ break_elab_rule ].
+  solve [ break_elab_rule; repeat process_eq_term (*TODO: why is this needed?*) ].
+  solve [ break_elab_rule; repeat process_eq_term (*TODO: why is this needed?*) ].
+  solve [ break_elab_rule; repeat process_eq_term (*TODO: why is this needed?*) ].
+  {
+     match goal with
+  | |- elab_rule _ (sort_rule _ _) _ => eapply elab_sort_rule; [ break_down_elab_ctx | solve_sublist ]
+  | |- elab_rule _ (term_rule _ _ _) _ => eapply elab_term_rule; [ break_down_elab_ctx | break_elab_sort | solve_sublist ]
+  | |- elab_rule _ (term_eq_rule _ _ _ _) _ => eapply eq_term_rule
+     end.
+     break_down_elab_ctx.
+     break_elab_sort.
+     solve[try_break_elab_term].
   simpl;
-    rewrite unfold_wf_term_dec.
-  break_dec_goal().
-  next_goal().
-  
-  
+   lazymatch goal with
+   | |- elab_term _ _ ?e ?ee ?t =>
+     tryif (is_evar e; is_evar ee) then shelve else eapply elab_term_conv
+   end.
+  eapply elab_term_by; [solve_in|].
 
+  eapply elab_args_cons_ex'; [ solve_len_eq | |].
 
-  {
-    simpl.
-    rewrite unfold_wf_term_dec.
-    next_goal().
-    rewrite unfold_wf_args_dec.
-    next_goal().
-    simpl; rewrite unfold_wf_term_dec.
-    next_goal().
-    {
-      simpl; rewrite unfold_wf_sort_dec.
-      next_goal().
-      simpl.
-      rewrite unfold_wf_args_dec.
-      next_goal().
-      rewrite unfold_wf_term_dec.
-      next_goal().
-      rewrite unfold_wf_args_dec.
-      next_goal().
-      {
-        cbn[with_names_from].
-        cbn[cat_lang_sub_r subst_lang_el_ty].
-        cbn [nth_tail named_list_lookup_err
-                      named_list_lookup
-              cat fst snd
-              String.eqb Ascii.eqb Bool.eqb].
-        simpl; rewrite unfold_wf_term_dec.
-        todo
-        next_goal().
-      {
-        simpl; rewrite unfold_wf_sort_dec.
-        next_goal().
-        simpl; rewrite unfold_wf_args_dec.
-        next_goal().
-        rewrite unfold_wf_term_dec.
-        next_goal().
-        rewrite unfold_wf_args_dec.
-        next_goal().
-        
-        simpl; rewrite unfold_wf_term_dec.
-      next_goal().
-      
-      rewrite unfold_wf_args_dec; rewrite ?eq_refl.
-      repeat ltac1:(timeout 2 ltac2:(break_dec_goal())).
-      repeat (first [ rewrite unfold_wf_sort_dec;
-                     repeat ltac1:(timeout 2 ltac2:(break_dec_goal()))
-                   | rewrite unfold_wf_term_dec;
-                     repeat ltac1:(timeout 2 ltac2:(break_dec_goal()))
-                   | rewrite unfold_wf_args_dec;
-                     repeat ltac1:(timeout 2 ltac2:(break_dec_goal()))
-             ]).
-      match!goal with [|-is_true(_==?e)]=> remember $e as x end.
-      means there is a weaken I don't want
-      vm_compute in Heqx.
-      cbn.
-      
-      break_dec_goal().
-  break_dec_goal().
-  break_dec_goal().
-      
-  
-    cbn[with_names_from term_args_elab nth_tail named_list_lookup_err
-              cat fst snd rec_stlc
-              String.eqb Ascii.eqb Bool.eqb apply_subst sort_subst exp_subst].
-    cbv[term_args_elab].
-    simpl.
-    break_dec_goal().
-  vm_compute; reflexivity.
-Qed.
+  simpl.
 
-  
-Derive elab_stlc
-       SuchThat (elab_lang stlc elab_stlc)
-       As elab_stlc_pf.
-Proof.
-  repeat (simpl; step_elab());
-    try (solve[repeat (simpl; step_elab())
-              | repeat(elab_term_by())]).
-  { repeat (elab_term_by()). }
-  { repeat (elab_term_by()). }
-  { repeat (elab_term_by()). }
   {
     eapply elab_term_conv.
+    eapply elab_term_by; [solve_in|].
+    eapply elab_args_cons_ex'; [ solve_len_eq | |].
+    solve[try_break_elab_term].
 
+    eapply elab_args_cons_im; [ | shelve ].
+    eapply elab_args_cons_ex'; [ solve_len_eq | |].
     {
-      elab_term_by().
-      {
-        elab_term_by().
-        elab_term_by().
-        elab_term_by().
-      }
-      {
-        elab_term_by(); repeat(simpl; step_elab()).
-        {
-          eapply elab_term_conv; repeat(simpl; step_elab()).
-          eapply Core.le_sort_refl'; repeat (simpl; step_elab()); try reflexivity.
-          symmetry.
-          eapply (@Core.le_term_by' "ty_subst_id"%string); repeat (simpl; step_elab()); reflexivity.
-        }
-        elab_term_by().    
-        step_elab().
-      }
-      { repeat (elab_term_by()). }
-      { step_elab(). }
-    }
-    { repeat (simpl;step_elab()).
-      
-      constructor.
-      repeat (simpl;step_elab()).
-      apply Core.wf_term_by';
-        repeat (simpl; step_elab()).
-      constructor; repeat (simpl; step_elab()).
-      constructor; repeat (simpl; step_elab()).
       simpl.
-      apply Core.wf_term_by';
-        repeat (simpl; step_elab()).
-      constructor.
-      repeat (simpl; step_elab()).
-      simpl.
-      eapply Core.wf_term_conv>[| repeat (simpl; step_elab())|].
-      repeat (simpl; step_elab()).
-      simpl.
+      eapply elab_term_conv.
+      eapply elab_term_by; [solve_in|].
+      eapply elab_args_cons_ex'; [ solve_len_eq | |].
       {
-        eapply Core.le_sort_refl'; repeat (cbn; step_elab()); try reflexivity.
-        symmetry.
-        eapply (@Core.le_term_by' "ty_subst_id"%string); repeat (cbn; step_elab()); reflexivity.
-      }
-    }
-    { 
-      eapply Core.le_sort_refl'; repeat (simpl; step_elab()); try reflexivity.
-      eapply Core.le_term_trans.
-      Focus 2.
-      eapply (@Core.le_term_by' "ty_subst_id"%string); repeat (simpl; step_elab()); reflexivity.
-      eapply Core.le_term_trans.
-
-      symmetry.
-      eapply (@Core.le_term_by' "ty_subst_cmp"%string); repeat (simpl; step_elab());
-      try reflexivity.
-      eapply Core.le_term_refl'; repeat (simpl; step_elab()); try reflexivity.
-      eapply (@Core.le_term_by' "wkn_snoc"%string); repeat (simpl; step_elab());
-      reflexivity.
-    }
-  }
-  {
-    apply elab_term_by'; repeat (simpl;step_elab()).
-    apply elab_term_by'; repeat (simpl;step_elab()).
-    eapply elab_term_conv.
-    solve [repeat (apply elab_term_by'; repeat (simpl;step_elab()))].
-    repeat (simpl; step_elab()).
-    {
-       eapply Core.le_sort_refl'; repeat (simpl; step_elab()); try reflexivity.
-       eapply (@Core.le_term_by' "->_subst"%string); repeat (simpl; step_elab()); reflexivity.
-    }
-    
-    solve [repeat (apply elab_term_by'; repeat (simpl;step_elab()))].
-    solve [repeat (apply elab_term_by'; repeat (simpl;step_elab()))].
-  }
-  {
-    solve [repeat (apply elab_term_by'; repeat (simpl;step_elab()))].
-  }
-  {    
-    solve [repeat (apply elab_term_by'; repeat (simpl;step_elab()))].
-  }
-  {
-    eapply elab_term_conv.
-    refine_elab '(Exp.con "lambda" [:: _; _; Exp.con "ty_subst" [:: Exp.var "A" ;Exp.var "g"; _; _]; _]).
-    elab_term_by().
-    eapply elab_term_conv.
-    {
-      elab_term_by().
-      {
-        solve [repeat (apply elab_term_by'; repeat (simpl;step_elab()))].
-      }
-      {
-        elab_term_by().
+        simpl.
         eapply elab_term_conv.
-        elab_term_by().
-        refine_elab '(Exp.con "ty_subst" [:: Exp.var "A" ;Exp.var "g"; _; _]).
-        elab_term_by().
-        step_elab().
-        apply Core.wf_sort_by'; repeat (simpl;step_elab()).
-         {
-          eapply Core.le_sort_refl'; repeat (simpl; step_elab()); try reflexivity.
-          simpl.
-          symmetry.
-          eapply (@Core.le_term_by' "ty_subst_cmp"%string); repeat (simpl; step_elab()); reflexivity.
-         }
-         simpl.
-         solve[repeat(elab_term_by())].
-         solve[repeat(elab_term_by())].
-      }
-      { 
-        solve[repeat(elab_term_by())].
-      }
-      { 
-        solve[repeat(elab_term_by())].
-      }
-    }
-    { repeat (simpl; step_elab()).
-      constructor; repeat (simpl; step_elab()).
-      simpl.
-        apply Core.wf_term_by'; repeat (simpl;step_elab()).
-        constructor; repeat (simpl; step_elab()).
-        constructor; repeat (simpl; step_elab()).
-        apply Core.wf_term_by'; repeat (simpl;step_elab()).
-        constructor; repeat (simpl; step_elab()).
-        eapply Core.wf_term_conv.
-        Focus 2.
-        apply Core.wf_term_by'; repeat (simpl;step_elab()).
-        repeat (simpl;step_elab()).
+        eapply elab_term_by; [solve_in|].
+        eapply elab_args_cons_im; [ | shelve ].
+        eapply elab_args_cons_im; [ | shelve ].
+        econstructor.
+
         {
-          eapply Core.le_sort_refl'; repeat (simpl; step_elab()); try  reflexivity.
-          symmetry.
-          eapply (@Core.le_term_by' "ty_subst_cmp"%string); repeat (simpl; step_elab()); reflexivity.
+          simpl.
+          sort_cong.
+          simpl.
+          term_refl.
+          simpl.
+          shelve.
         }
+      }
+      {
+        eapply elab_args_cons_ex'; [ solve_len_eq | |].
+        {
+          simpl.
+          eapply elab_term_conv.
+          eapply elab_term_by; [solve_in|].
+          {
+            eapply elab_args_cons_ex'; [ solve_len_eq | |].
+            {
+              simpl.
+              eapply elab_term_var; solve_in.
+            }
+            
+            eapply elab_args_cons_ex'; [ solve_len_eq | |].
+            {
+              simpl.
+              eapply elab_term_conv.
+              eapply elab_term_by; [solve_in|].
+              eapply elab_args_cons_im; [ | shelve ].
+              eapply elab_args_cons_im; [ | shelve ].
+              constructor.
+              
+              simpl.
+              sort_cong; term_refl.
+            }
+            eapply elab_args_cons_im; [ | shelve ].
+            eapply elab_args_cons_im; [ | shelve ].
+            eapply elab_args_cons_im; [ | shelve ].
+            constructor.
+          }
+
+          simpl.
+          sort_cong; term_refl.
+        }
+        
+        eapply elab_args_cons_im; [ | shelve ].
+        eapply elab_args_cons_im; [ | shelve ].
+        eapply elab_args_cons_im; [ | shelve ].
+        constructor.
+      }
+      {
+        simpl.
+        sort_cong; term_refl.
+      }
     }
-     {
-      eapply Core.le_sort_refl'; repeat (simpl; step_elab()); try reflexivity.
-      eapply Core.le_term_trans.
-      symmetry.
-      eapply (@Core.le_term_by' "ty_subst_cmp"%string); repeat (simpl; step_elab()); reflexivity.
-      symmetry.
-      eapply Core.le_term_trans.
-      symmetry.      
-      eapply (@Core.le_term_by' "ty_subst_cmp"%string); repeat (simpl; step_elab()); reflexivity.
-      eapply Core.le_term_refl'; repeat (simpl; step_elab()); try reflexivity.
-      symmetry.
-      eapply Core.le_term_trans.
-      eapply (@Core.le_term_by' "wkn_snoc"%string); repeat (simpl; step_elab()); reflexivity.
-      reflexivity.
-     }
-     { 
-       solve[repeat(elab_term_by())].
-     }
-     { 
-       solve[repeat(elab_term_by())].
-     }
-     {
-       solve[repeat(simpl; step_elab())].
-     }
-     {
-       solve[repeat(simpl; step_elab())].
-     }
-     {
-       eapply Core.le_sort_refl'; repeat (simpl; step_elab()); try reflexivity.
-       symmetry.
-       eapply (@Core.le_term_by' "->_subst"%string); repeat (simpl; step_elab()); reflexivity.
-     }
-  }
-Qed.
-  
-Instance elab_stlc_inst : Elaborated stlc :=
-  {
-  elaboration := elab_stlc;
-  elab_pf := elab_stlc_pf;
-  }.
-
-(* Some starter code for an STLC-specific partial recognizer
-
-TODO: do I want to try this approach?
-Fixpoint unfold_stlc_subst_list (subst_list : list (Exp.exp * Exp.exp * Exp.exp))  (e : Exp.exp) : Exp.exp :=
-  match subst_list with
-  | [::] => e
-  | (g,G',G)::sl => unfold_stlc_subst_list sl (Exp.con "ty_subst" [:: e; g; G'; G])
-  end.
-
-Lemma unfold_var_injective sl1 sl2 x1 x2
-  : (unfold_stlc_subst_list sl1 (Exp.var x1) == unfold_stlc_subst_list sl2 (Exp.var x2))
-    = (sl1 == sl2) && (x1 == x2).
-Proof.
-  revert sl2; induction sl1; intro sl2; destruct sl2; ltac1:(break); simpl; auto.
-  admit.
-  admit.
-  Search foldl.
-Admitted.
-
-Fixpoint hnf_stlc_ty (subst_list : list (Exp.exp * Exp.exp * Exp.exp))  (e : Exp.exp) : Exp.exp :=
-  match e with
-  | (Exp.con "->" args) => Exp.con "->" (map (hnf_stlc_ty subst_list) args)
-  | (Exp.con "ty_subst" [:: Exp.con "->" [:: B; A; G1']; g; G'; G]) =>
-    let hnf := hnf_stlc_ty ((g,G',G)::subst_list) in
-    Exp.con "->" [:: hnf B; hnf A; G]
-  | _ => unfold_stlc_subst_list subst_list e
-  end.
-
-Definition stlc_type_eq t1 t2 :=
-  (hnf_stlc_ty [::] t1) == (hnf_stlc_ty [::] t2).
-
-(*
-Lemma hnf_stlc_ty_con n s sb : exists n' s', hnf_stlc_ty sb (Exp.con n s) = Exp.con n' s'.
-Admitted.
-*)
-
-Lemma stlc_type_eq_constr_inv n s x
-  : ~~ (stlc_type_eq (Exp.con n s) (Exp.var x)).
-Proof using .
-  ltac1:(apply /negP).
-  unfold stlc_type_eq.
-  ltac1:(move /eqP).
-  repeat (simpl; ltac1:(case_match;try by inversion)).
-Qed.
-
-Lemma stlc_type_eq_sym a b
-  : (stlc_type_eq a b) = stlc_type_eq b a.
-Proof using .
-  apply eq_sym.
-Qed.
-
-Lemma stlc_type_eq_recognizes c e1 e2 G
- : Core.wf_term (strip_args elab_stlc) c e1 (Exp.srt "ty" [:: G]) ->
-   Core.wf_term (strip_args elab_stlc) c e2 (Exp.srt "ty" [:: G]) ->
-   stlc_type_eq e1 e2 ->
-   Core.le_term (strip_args elab_stlc) c (Exp.srt "ty" [:: G]) e1 e2.
-Proof.
-  unfold stlc_type_eq.
-  generalize (@nil (Exp.exp *Exp.exp*Exp.exp)).
-  revert e2.
-  induction e1; intro e2; destruct e2.
-  {
-    intros l _ _.
-    intro stlceq.
-    cbn in stlceq.
-    simpl in stlceq.
-    rewrite !unfold_var_injective in stlceq.
-    ltac1:(break).
-    ltac1:(move: stlceq=> /eqP => ->).
-    reflexivity.
-  }    
-  {
-    intros sl _ _.
-    ltac1:(move /negPn).
-    admit.
-  }    
-  { admit. }  
-  {
-    intros wf1 wf2.
-    unfold stlc_type_eq.
-    match! goal with
-      [|- is_true(?a == ?b) -> _]=>
-      remember $a as l_hnf;
-        remember $b as r_hnf
-    end.
-    ltac1:(case neq: (n=="ty_subst"%string)).
-    {
-      ltac1:(move: neq => /eqP neq).
-      rewrite neq in Heql_hnf.
-      simpl in Heql_hnf.
-      rewrite neq in wf1.
-      
-      
-    issue: ty_substs
-    repeat (simpl; ltac1:(case_match)).
-  unfold stlc_type_eq in ty_eq.
-  rewrite !hnf_stlc_ty_con in ty_eq.
-  simpl in ty_eq.
-  {
-    destruct n0; try (inversion ty_eq).
-  intro wft; induction wft.
-  {
     
+    eapply elab_args_cons_im; [ | shelve ].
+    eapply elab_args_cons_im; [ | shelve ].
+    constructor.
 
-Fixpoint elab_lam_term (e : exp) (t : Exp.sort) : option Exp.exp :=
-  match e, t with
-  | con "lambda" [:: e], scon "el" [:: ty; G] =>
-    match simpl_stlc_ty
-  | _,_ => None
-  end.
+    {
+      simpl.
+      sort_cong; simpl.
+      term_refl.
+      instantiate (2:= {{e#"ty_subst" %"G'" %"G" %"g" %"A"}}).
+      instantiate (1:= {{e#"ty_subst" %"G'" %"G" %"g" %"B"}}).
+      compute_everywhere (nth_tail 1 stlc_elab).
+      by_reduction.
+      
+      (*TODO: this is unwieldly, curr. have to write out instantiation for a; 
+        need tactics (e.g. rewrite) that work w/ evars,
+        or a way to better clear them before I get here.
+
+        remainder of proof needed:    
+        fill ?a with (ty_subst g B), reduce
+       *)
+    }
+  }
+
+  break_down_elab_args.
+
+  sort_cong; process_eq_term.
+
+  Unshelve.
+  all: try cleanup_auto_elab.
+  all: try apply eq_term_refl.
+  all: try cleanup_auto_elab.
+  {
+    unshelve (repeat (constructor;[|try cleanup_auto_elab; shelve])).
+    2: constructor.
+    simpl.
+    eapply wf_term_conv.
+    eapply wf_term_by; [solve_in|].
+    eapply wf_args_cons.
+    simpl.
+    {
+      eapply wf_term_conv.
+      eapply wf_term_var; [solve_in].
+      sort_cong; by_reduction.
+    }
+    cleanup_auto_elab.
+
+    simpl.
+    sort_cong; term_refl.
+  }
+  {
+    unshelve (repeat (constructor;[|try cleanup_auto_elab; shelve])).
+
+    simpl.
+    {
+      eapply wf_term_conv.
+      eapply wf_term_var; [solve_in].
+      sort_cong; by_reduction.
+    }
+
+    
+    cleanup_auto_elab.
+  }
+  {
+      compute_everywhere (nth_tail 1 stlc_elab).
+      by_reduction.
+  }
+  
+  {
+    unshelve (repeat (constructor;[|try cleanup_auto_elab; shelve])).
+
+    simpl.
+    {
+      eapply wf_term_conv.
+      eapply wf_term_by; [solve_in|].
+      constructor.
+      {
+        simpl.
+        eapply wf_term_conv.
+        eapply wf_term_by; [solve_in|].
+        
+        cleanup_auto_elab.
+        simpl.
+        sort_cong; by_reduction.
+      }
+      cleanup_auto_elab.
+      sort_cong; by_reduction.
+    }
+    constructor.
+  }
+  {
+    unshelve (repeat (constructor;[|try cleanup_auto_elab; shelve])).
+    simpl.
+    {
+      eapply wf_term_conv.
+      eapply wf_term_by; [solve_in|].
+      cleanup_auto_elab.
+
+      simpl.
+      sort_cong; by_reduction.
+    }
+    cleanup_auto_elab.
+    
+  }
+  Unshelve.
+  all: try cleanup_auto_elab.
+
+  simpl.
+  cleanup_auto_elab.
+  }
+Qed.  
+     
+(*TODO: currently re-proves subst_lang correct;
+  develop machinery to reuse
 *)
